Check Program

coq-proof/ProgramDefs.v
@@ -21,24 +21,24 @@ From PUnits Require Import VarDecl.
 From PUnits Require Import ExpressionDefs.
 From PUnits Require Import StatementDefs.
 
-(* ======================================================= *)
+(* Program P in the language. *)
 Inductive Program : Type :=
-  | program : Field_Declarations -> Statements -> Program.
+  | program : Variable_Declarations -> Statements -> Program.
 Tactic Notation "prog_cases" tactic(first) ident(c) :=
   first;
   [ Case_aux c "program"
   ].
 Hint Constructors Program : pUnitsHintDatabase.
 
-Notation "{ fds s }" := (program fds s) (at level 1).
+Notation "{ vds s }" := (program vds s) (at level 1).
 
 (* ======================================================= *)
 Reserved Notation "'prog:' g '|-' p 'in' post_gamma" (at level 40).
 Inductive prog_has_type : Gamma -> Program -> Gamma -> Prop :=
-  | T_Program : forall (g post_gamma : Gamma) (fds : Field_Declarations) (s : Statements),
-    fds: g |- fds in post_gamma ->
+  | T_Program : forall (g post_gamma : Gamma) (vds : Variable_Declarations) (s : Statements),
+    vds: g |- vds in post_gamma ->
     stmt: post_gamma |- s ->
-    prog: g |- program fds s in post_gamma
+    prog: g |- program vds s in post_gamma
 where "'prog:' g '|-' p 'in' post_gamma" := (prog_has_type g p post_gamma).
 Tactic Notation "prog_has_type_cases" tactic(first) ident(c) :=
   first;
@@ -49,24 +49,24 @@ Hint Constructors prog_has_type : pUnitsHintDatabase.
 (* ======================================================= *)
 Reserved Notation " p1 'prog==>' p2 " (at level 8).
 Inductive prog_small_step : prod StackFrame Program -> prod StackFrame Program -> Prop :=
-  | ST_PROG_VarDecl_Step : forall h h' fds fds' s,
-    ( h, fds ) fds==> ( h', fds' ) ->
-    ( h, program fds s ) prog==> ( h', program fds' s )
-  | ST_PROG_Statementss_Step : forall h h' s s',
-    ( h, s ) stmt==> ( h', s' ) ->
-    ( h, program FD_Empty s ) prog==> ( h', program FD_Empty s' )
+  | ST_PROG_VarDecl_Step : forall (f f' : StackFrame) (vds vds' : Variable_Declarations) (s : Statements),
+    ( f, vds ) vds==> ( f', vds' ) ->
+    ( f, program vds s ) prog==> ( f', program vds' s )
+  | ST_PROG_Statements_Step : forall (f f' : StackFrame) (s s' : Statements),
+    ( f, s ) stmt==> ( f', s' ) ->
+    ( f, program VD_Empty s ) prog==> ( f', program VD_Empty s' )
 where " p1 'prog==>' p2 " := (prog_small_step p1 p2).
 Tactic Notation "prog_small_step_cases" tactic(first) ident(c) :=
   first;
   [ Case_aux c "ST_PROG_VarDecl_Step"
-  | Case_aux c "ST_PROG_Statementss_Step"
+  | Case_aux c "ST_PROG_Statements_Step"
   ].
 Hint Constructors prog_small_step : pUnitsHintDatabase.
 
 (* ======================================================= *)
 (* step is deterministic *)
 Theorem prog_small_step_deterministic:
-  forall p p1 p2,
+  forall (p p1 p2 : prod StackFrame Program),
     p prog==> p1 ->
     p prog==> p2 ->
     p1 = p2.
@@ -76,46 +76,46 @@ Proof.
   prog_small_step_cases (induction Hp1) Case.
   Case "ST_PROG_VarDecl_Step".
     intros p2 Hp2; inversion Hp2; subst.
-      assert ((h', fds') = (h'0, fds'0)) as HfdsEQ. eapply fds_small_step_deterministic.
-        apply H. apply H4. inversion HfdsEQ; subst. reflexivity.
+      assert ((f', vds') = (f'0, vds'0)) as HvdsEQ. eapply vds_small_step_deterministic.
+        apply H. apply H4. inversion HvdsEQ; subst. reflexivity.
       inversion H.
-  Case "ST_PROG_Statementss_Step".
+  Case "ST_PROG_Statements_Step".
     intros p2 Hp2; inversion Hp2; subst.
       inversion H4.
-      assert ((h', s') = (h'0, s'0)) as HsEQ. eapply stmt_small_step_deterministic.
+      assert ((f', s') = (f'0, s'0)) as HsEQ. eapply stmt_small_step_deterministic.
         apply H. apply H3. inversion HsEQ; subst. reflexivity.
 Qed.
 
 (* ======================================================= *)
 Inductive prog_normal_form : Program -> Prop :=
-  | V_PROG_NF : prog_normal_form (program FD_Empty STMT_Empty).
+  | V_PROG_NF : prog_normal_form (program VD_Empty STMT_Empty).
 
 (* ======================================================= *)
-Theorem prog_progress : forall (g1 g2 : Gamma) (h : StackFrame) (p : Program),
+Theorem prog_progress : forall (g1 g2 : Gamma) (f : StackFrame) (p : Program),
   prog: g1 |- p in g2 ->
-  gf: g2 |- h OK ->
-  prog_normal_form p \/ exists (h' : StackFrame) (p' : Program), (h, p) prog==> (h', p').
+  gf: g2 |- f OK ->
+  prog_normal_form p \/ exists (f' : StackFrame) (p' : Program), (f, p) prog==> (f', p').
 Proof.
   (* by induction on typing of prog *)
-  intros g1 g2 h p HT HGH.
+  intros g1 g2 f p HT HGF.
   prog_has_type_cases (induction HT) Case; subst.
   Case "T_Program".
-    assert (FD_Normal_Form fds \/ exists heap' fds', (h, fds) fds==> (heap', fds')).
-      eapply fds_progress. apply H.
-    assert (STMT_Normal_Form s \/ exists (h' : StackFrame) (s' : Statements), (h, s) stmt==> (h', s')).
-      eapply stmt_progress. apply H0. apply HGH.
+    assert (VD_Normal_Form vds \/ exists (f' : StackFrame) (vds' : Variable_Declarations), (f, vds) vds==> (f', vds')).
+      eapply vds_progress. apply H.
+    assert (STMT_Normal_Form s \/ exists (f' : StackFrame) (s' : Statements), (f, s) stmt==> (f', s')).
+      eapply stmt_progress. apply H0. apply HGF.
     destruct H1; subst.
-    (* Case : FD is normal form *)
+    (* Case : vds is normal form *)
       destruct H2; subst.
       (* Case : STMT is normal form *)
         destruct H1; subst. destruct H2; subst. left. apply V_PROG_NF.
       (* Case : STMT can take a step *)
-        destruct H1; subst. right. destruct H2 as [h']. destruct H1 as [s'].
-        exists h'. exists (program FD_Empty s').
-        apply ST_PROG_Statementss_Step. apply H1.
-    (* Case : FD can take a step *)
-      destruct H1 as [h']. destruct H1 as [fds']. right.
-      exists h'. exists (program fds' s).
+        destruct H1; subst. right. destruct H2 as [f']. destruct H1 as [s'].
+        exists f'. exists (program VD_Empty s').
+        apply ST_PROG_Statements_Step. apply H1.
+    (* Case : vds can take a step *)
+      destruct H1 as [f']. destruct H1 as [vds']. right.
+      exists f'. exists (program vds' s).
       apply ST_PROG_VarDecl_Step. apply H1.
 Qed.
 
@@ -123,49 +123,50 @@ Qed.
 
 Definition Gamma_Extend_Prog (g : Gamma) (p : Program) : Gamma :=
   match p with
-  | program fds s => Gamma_Extend_Fields g fds
+  | program vds s => Gamma_Extend_Variables g vds
   end.
 
 (* ======================================================= *)
-Theorem prog_preservation : forall (g post_gamma : Gamma) (h h' : StackFrame) (p p' : Program),
+Theorem prog_preservation : forall (g post_gamma : Gamma) (f f' : StackFrame) (p p' : Program),
   prog: g |- p in post_gamma ->
-  gf: post_gamma |- h OK ->
-  (h, p) prog==> (h', p') ->
-  gf: post_gamma |- h' OK /\ prog: (Gamma_Extend_Prog g p) |- p' in post_gamma.
+  gf: post_gamma |- f OK ->
+  (f, p) prog==> (f', p') ->
+  gf: post_gamma |- f' OK /\ prog: (Gamma_Extend_Prog g p) |- p' in post_gamma.
 Proof.
   (* by induction on typing of program *)
-  intros g post_gamma h h' p p' HT HGH HS.
-  (* we prove for programs typed starting from empty gamma, rather than all possible gamma *)
+  intros g post_gamma f f' p p' HT HGF HS.
+  (* we prove for programs typed starting from empty gamma, rather than all
+     possible gamma *)
   remember empty_gamma as Gamma.
-  generalize dependent p'. generalize dependent h'.
-  prog_has_type_cases (induction HT) Case; intros h' p' HS; subst.
+  generalize dependent p'. generalize dependent f'.
+  prog_has_type_cases (induction HT) Case; intros f' p' HS; subst.
   Case "T_Program".
-    destruct p' as [fds' s'].
+    destruct p' as [vds' s'].
     prog_small_step_cases (inversion HS) SCase; subst.
     SCase "ST_PROG_VarDecl_Step".
       inversion H2; subst.
       unfold Gamma_Extend_Prog. simpl.
-      eapply fds_preservation in H.
+      eapply vds_preservation in H.
       destruct H.
         split.
-        (* first prove that post_gamma |- h' OK *)
+        (* first prove that post_gamma |- f' OK *)
           apply H.
         (* then prove that prog: (Gamma_Extend_Prog empty_gamma p) |- p' in post_gamma. *)
           apply T_Program.
             apply H1.
             apply H0.
-        apply HGH.
+        apply HGF.
         apply H2.
-    SCase "ST_PROG_Statementss_Step".
-      simpl. (* in statement step, the input gamma to type p' does not change *)
-        eapply stmt_preservation in H0.
+    SCase "ST_PROG_Statements_Step".
+      (* in statement step, the input gamma to type check p' does not change *)
+      simpl. eapply stmt_preservation in H0.
         split.
-        (* first prove that post_gamma |- h' OK *)
+        (* first prove that post_gamma |- f' OK *)
           apply H0.
-        (* then prove that prog: g |- {FD_Empty s'} in post_gamma *)
+        (* then prove that prog: g |- {VD_Empty s'} in post_gamma *)
           apply T_Program.
             apply H.
             apply H0.
-        apply HGH.
+        apply HGF.
         apply H2.
 Qed.
